compiler/bootstrap/translation/printingProgScript.sml
@@ -1,0 +1,89 @@
+(*
+  Translate the pretty printing functions for the REPL
+*)
+
+open preamble ml_translatorLib ml_translatorTheory
+     sexp_parserProgTheory std_preludeTheory printTweaksTheory
+
+val _ = set_grammar_ancestry ["infer","misc"];
+
+val _ = new_theory "printingProg"
+
+val _ = translation_extends "sexp_parserProg";
+
+val _ = ml_translatorLib.ml_prog_update (ml_progLib.open_module "printingProg");
+
+val RW = REWRITE_RULE
+
+val _ = add_preferred_thy "-";
+
+val NOT_NIL_AND_LEMMA = Q.prove(
+  `(b <> [] /\ x) = if b = [] then F else x`,
+  Cases_on `b` THEN FULL_SIMP_TAC std_ss []);
+
+val extra_preprocessing = ref [MEMBER_INTRO,MAP];
+
+val matches = ref ([]: term list);
+
+fun def_of_const tm = let
+  val res = dest_thy_const tm handle HOL_ERR _ =>
+              failwith ("Unable to translate: " ^ term_to_string tm)
+  val name = (#Name res)
+  fun def_from_thy thy name =
+    DB.fetch thy (name ^ "_pmatch") handle HOL_ERR _ =>
+    DB.fetch thy (name ^ "_def") handle HOL_ERR _ =>
+    DB.fetch thy (name ^ "_DEF") handle HOL_ERR _ =>
+    DB.fetch thy (name ^ "_thm") handle HOL_ERR _ =>
+    DB.fetch thy name
+  val def = def_from_thy (#Thy res) name handle HOL_ERR _ =>
+            failwith ("Unable to find definition of " ^ name)
+
+  val def = def |> RW (!extra_preprocessing)
+                |> CONV_RULE (DEPTH_CONV BETA_CONV)
+                (* TODO: This ss messes up defs containing if-then-else
+                with constant branches
+                |> SIMP_RULE bool_ss [IN_INSERT,NOT_IN_EMPTY]*)
+                |> REWRITE_RULE [NOT_NIL_AND_LEMMA]
+  in def end
+
+val _ = (find_def_for_const := def_of_const);
+
+val _ = use_long_names:=true;
+
+val _ = ml_translatorLib.use_string_type true;
+
+val r = translate typeDecToPPTheory.con_x_i_pat_def;
+val r = translate addTypePPTheory.add_pp_decs_def;
+
+Triviality OPT_MAP_I:
+  ∀g ls. OPT_MMAP I (MAP g ls) = OPT_MMAP g ls
+Proof
+  Induct_on ‘ls’ \\ fs [listTheory.OPT_MMAP_def]
+QED
+
+val r = translate
+  (addPrintValsTheory.inf_t_to_ast_t_def
+   |> SIMP_RULE std_ss [Once (GSYM OPT_MAP_I)]);
+
+val r = translate addPrintValsTheory.print_of_val_def;
+
+val r = translate (DefnBase.one_line_ify NONE addPrintValsTheory.nsContents_def);
+
+val r = translate
+  (printTweaksTheory.add_print_features_def
+   |> SIMP_RULE (srw_ss()) [inferTheory.init_infer_state_def]);
+
+val lemma = prove(“printtweaks_add_print_features_side x y = T”,
+  rw [fetch "-" "printtweaks_add_print_features_side_def"]
+  \\ irule (inferProgTheory.infer_d_side_thm |> CONJUNCT2) \\ fs []
+  \\ irule (inferPropsTheory.infer_d_wfs |> CONJUNCT2) \\ fs []
+  \\ first_x_assum $ irule_at Any \\ fs [])
+  |> update_precondition;
+
+val () = Feedback.set_trace "TheoryPP.include_docs" 0;
+
+val _ = ml_translatorLib.ml_prog_update (ml_progLib.close_module NONE);
+
+val _ = (ml_translatorLib.clean_on_exit := true);
+
+val _ = export_theory();
